examples/ssr/SystemF_CBV.v
@@ -1,6 +1,6 @@
 (** * Normalization of Call-By-Value System F *)
 
-Require Import Autosubst MMap.
+Require Import Autosubst.
 Require Import ssreflect ssrfun ssrbool eqtype ssrnat seq.
 
 Set Implicit Arguments.
@@ -23,7 +23,7 @@ Inductive term :=
 
 (** **** Substitution Lemmas *)
 
-Instance VarConstr_type : VarConstr type. derive. Defined.
+Instance Ids_type : Ids type. derive. Defined.
 Instance Rename_type : Rename type. derive. Defined.
 Instance Subst_type : Subst type. derive. Defined.
 
@@ -31,7 +31,7 @@ Instance SubstLemmas_type : SubstLemmas type. derive. Qed.
 
 Instance HSubst_term : HSubst type term. derive. Defined.
 
-Instance VarConstr_term : VarConstr term. derive. Defined.
+Instance Ids_term : Ids term. derive. Defined.
 Instance Rename_term : Rename term. derive. Defined.
 Instance Subst_term : Subst term. derive. Defined.
 
@@ -44,9 +44,9 @@ Instance SubstLemmas_term : SubstLemmas term. derive. Qed.
 
 Inductive eval : term -> term -> Prop :=
 | eval_beta (A : type) (s t u1 u2 v : term) :
-    eval s (Abs A u1) -> eval t u2 -> eval (u1.[u2.:Var]) v -> eval (App s t) v
+    eval s (Abs A u1) -> eval t u2 -> eval (u1.[u2/]) v -> eval (App s t) v
 | eval_tbeta (B : type) (s A v : term) :
-    eval s (TAbs A) -> eval (A.|[B.:Var]) v -> eval (TApp s B) v
+    eval s (TAbs A) -> eval (A.|[B/]) v -> eval (TApp s B) v
 | eval_abs (A : type) (s : term) :
     eval (Abs A s) (Abs A s)
 | eval_tabs (A : term) :
@@ -56,12 +56,12 @@ Hint Resolve eval_abs eval_tabs.
 (** **** Syntactic typing *)
 
 Definition ctx := seq type.
-Local Notation "Gamma `_ i" := (nth (Var 0) Gamma i).
+Local Notation "Gamma `_ i" := (nth (ids 0) Gamma i).
 Definition raise (Gamma : ctx) := [seq A.[ren (+1)] | A <- Gamma].
 
 Inductive has_type (Gamma : ctx) : term -> type -> Prop :=
 | ty_var (x : var) :
-    x < size Gamma -> has_type Gamma (Var x) Gamma`_x
+    x < size Gamma -> has_type Gamma (TeVar x) Gamma`_x
 | ty_abs (A B : type) (s : term) :
     has_type (A :: Gamma) s B ->
     has_type Gamma (Abs A s) (Arr A B)
@@ -74,7 +74,7 @@ Inductive has_type (Gamma : ctx) : term -> type -> Prop :=
     has_type Gamma (TAbs s) (All A)
 | ty_tapp (A B : type) (s : term) :
     has_type Gamma s (All A) ->
-    has_type Gamma (TApp s B) A.[B.:Var].
+    has_type Gamma (TApp s B) A.[B/].
 
 (** **** Semantic typing *)
 
@@ -85,9 +85,9 @@ Fixpoint V (A : type) (rho : var -> term -> Prop) (v : term) {struct A} : Prop :
   match A with
     | TyVar X => eval v v /\ rho X v
     | Arr A B => exists A' : type, exists2 s : term, v = Abs A' s &
-        forall u, V A rho u -> L (V B rho) s.[u.:Var]
+        forall u, V A rho u -> L (V B rho) s.[u/]
     | All A => exists2 s : term, v = TAbs s &
-        forall i (B : type), L (V A (i .: rho)) s.|[B.:Var]
+        forall i (B : type), L (V A (i .: rho)) s.|[B/]
   end.
 Notation E A rho := (L (V A rho)).
 
@@ -113,19 +113,19 @@ Proof.
 Qed.
 
 Lemma V_ren A rho s xi :
-  V A.[ren xi] rho s <-> V A (xi >> rho) s.
+  V A.[ren xi] rho s <-> V A (xi >>> rho) s.
 Proof.
   elim: A rho s xi => //=.
   - move=> A ih1 B ih2 rho v xi. split=> -[A'[s->h]];
      (do 2 eexists) => // t /ih1/h[u ev]/ih2 ih; by exists u.
-  - move=> A ih rho s xi; autosubst.
-    split=> -[s' -> h]; eexists; autosubst=> P B; move: {h} (h P B) => [v ev].
-    + move=> /ih {ih} ih. exists v => //. by autosubst in ih.
-    + move=> h. exists v => //. apply/ih. by autosubst.
+  - move=> A ih rho s xi; asimpl.
+    split=> -[s' -> h]; eexists => //; asimpl=> P B; move: {h} (h P B) => [v ev].
+    + move=> /ih {ih} ih. exists v => //. by asimpl in ih.
+    + move=> h. exists v => //. apply/ih. autosubst.
 Qed.
 
 Lemma E_ren A rho s xi :
-  E A.[ren xi] rho s <-> E A (xi >> rho) s.
+  E A.[ren xi] rho s <-> E A (xi >>> rho) s.
 Proof.
   split=> -[v ev /V_ren h]; by exists v.
 Qed.
@@ -138,11 +138,11 @@ Proof.
   - move=> A ih1 B ih2 rho v sigma /=. split=> -[A' [s->h]];
       (do 2 eexists) => // t /ih1/h[u ev]/ih2 ih; by exists u.
   - move=> A ih rho v sigma. split;
-      autosubst; move=> [s->{v}h]; eexists=> [//|P B].
+      asimpl; move=> [s->{v}h]; eexists=> [//|P B].
     + move: (h P B) => [v ev /ih hv]. exists v => //.
-      apply: eq_V hv => -[|X] //= u. by intuition. move=> _. exact: V_ren.
+      apply: eq_V hv => -[|X] //= u. by intuition. move=> _. asimpl. exact: V_ren.
     + move: (h P B) => [v ev hv]. exists v => //. apply/ih.
-      apply: eq_V hv => -[|X] //= u. by intuition.
+      apply: eq_V hv => -[|X] //= u. by intuition. asimpl.
       split => [p|/V_ren//]. by apply/V_ren.
 Qed.
 
@@ -156,14 +156,14 @@ Proof.
   elim=> {Gamma s A} [Gamma x xe|Gamma A B s _ ih|Gamma A B s t _ ih1 _ ih2|
                       Gamma A s _ ih|Gamma A B s _ ih] delta sigma rho l.
   - exact: l.
-  - eexists; first by autosubst. (do 2 eexists)=> [//|t vt]. autosubst.
+  - eexists; first by autosubst. (do 2 eexists)=> [//|t vt]. asimpl.
     apply: ih=> -[_/=|x/l//]. exact: V_to_E.
   - case: (ih1 delta _ _ l) => {ih1} /= v ev1 [A' [u eq ih1]]; subst v.
     case: (ih2 delta _ _ l) => {ih2} v ev2 ih2.
     case: (ih1 _ ih2) => {ih1} w ev3 ih1. exists w => //.
     exact: eval_beta ev1 ev2 ev3.
-  - apply: V_to_E. eexists=> [//=|P B]. autosubst. apply: ih => x /=.
-    rewrite size_map => wf. rewrite (nth_map (Var 0)) //. apply/E_ren. exact: l.
+  - apply: V_to_E. eexists=> [//=|P B]. asimpl. apply: ih => x /=.
+    rewrite size_map => wf. rewrite (nth_map (ids 0)) //. apply/E_ren. exact: l.
   - move: (ih delta _ _ l) => [v ev1 {ih} /=[s' eq ih]]; subst v.
     specialize (ih (V B rho) B.[delta]). move: ih => [v ev2 ih]. exists v.
     exact: eval_tbeta ev1 ev2. apply/V_subst. apply: eq_V ih => -[|x] //=.
@@ -177,7 +177,7 @@ Definition nilA : var -> term -> Prop := fun _ _ => False.
 Corollary soundness_nil s A :
   has_type [::] s A -> E A nilA s.
 Proof.
-  move=> h. cut (E A nilA s.|[Var].[Var]). by autosubst. exact: (soundness h).
+  move=> h. cut (E A nilA s.|[ids].[ids]). autosubst. exact: (soundness h).
 Qed.
 
 Corollary normalization s A :
@@ -187,7 +187,7 @@ Proof.
 Qed.
 
 Corollary consistency s :
-  ~has_type [::] s (All (Var 0)).
+  ~has_type [::] s (All (TyVar 0)).
 Proof.
   move=> /soundness_nil[v _ /= [t {s v} _ /(_ (fun _ => False) (TyVar 0))]].
   by move=> [s {t} _ []].
@@ -197,9 +197,9 @@ Qed.
 
 Inductive step : term -> term -> Prop :=
 | step_beta (A : type) (s s' t : term) :
-    s' = s.[t.:Var] -> step (App (Abs A s) t) (s')
+    s' = s.[t/] -> step (App (Abs A s) t) (s')
 | step_tbeta (B : type) s s' :
-    s' = s.|[B.:Var] -> step (TApp (TAbs s) B) s'
+    s' = s.|[B/] -> step (TApp (TAbs s) B) s'
 | step_app1 s s' t :
     step s s' -> step (App s t) (App s' t)
 | step_app2 s t t' :
@@ -210,7 +210,11 @@ Inductive step : term -> term -> Prop :=
 Lemma substitutivity s t :
   step s t -> forall sigma tau, step s.|[tau].[sigma] t.|[tau].[sigma].
 Proof.
-  elim=> /=; constructor; subst; autosubst.
+  induction 1; constructor; subst; autosubst.
+Restart.
+  induction 1; asimpl; constructor; subst; trivial.
+  - autosubst.
+  - autosubst.
 Qed.
 
 Lemma substitutivity' s t :
