theories/Autosubst/MMap.v
@@ -1,0 +1,137 @@
+(**
+  Apply a function to all instances of a type A occuring in a type B.
+  This is used to implement term structures with containers, e.g.
+
+  Inductive term := C (xs : list term)
+
+  By default we provide mmap instances for option, list, pair and
+  the codomain of a function. For additional inductive types, there is
+  a derive tactic to generate new mmap instances.
+*)
+Require Import Basics.
+
+Class MMap (A B: Type) := mmap : (A -> A) -> B -> B.
+Arguments mmap {A B _} f !s /.
+
+(**
+  Extensionality for mmap. This Lemma is uninteresting, as it is implied by
+  functional extensionality. However, instances of this class should be
+  transparent and take the proof of [[forall t, f t = gt]] as a non-recursive
+  argument. This is sufficient to allow the fixpoint checker to lift proofs
+  over mmap.
+*)
+Class MMapExt (A B : Type) `{MMap A B} := 
+  mmap_ext : forall f g,
+    (forall t, f t = g t) -> forall s, mmap f s = mmap g s.
+Arguments mmap_ext {A B _ _ f g} H s.
+
+Class MMapLemmas (A B : Type) `{MMap A B} := {
+  mmap_id x : mmap id x = x;
+  mmap_comp f g x : mmap f (mmap g x) = mmap (g >>> f) x
+}.
+
+(** MMap Lemmas *)
+
+Section LemmasForMMap.
+
+Context {A B : Type}.
+Context {MMap_Inst : MMap A B} {MMapLemmas_Inst : MMapLemmas A B}.
+
+Lemma mmap_idX : mmap id = id.
+Proof. f_ext. exact mmap_id. Qed.
+
+Lemma mmap_compX f g : mmap f >>> mmap g = mmap (f >>> g).
+Proof. f_ext. apply mmap_comp. Qed.
+
+Lemma mmap_compR {C} f g (h : _ -> C) :
+  mmap f >>> mmap g >>> h = mmap (f >>> g) >>> h.
+Proof. now rewrite <- mmap_compX. Qed.
+
+End LemmasForMMap.
+
+(** Identity Instance *)
+
+Section MMapId.
+Context {A : Type}.
+Global Instance MMap_refl : MMap A A := id.
+Global Instance MMapLemmas_refl : MMapLemmas A A. now constructor. Qed.
+Global Instance MMapExt_refl : MMapExt A A. hnf. tauto. Defined.
+End MMapId.
+
+Arguments MMap_refl _ _ f /.
+
+Lemma mmap_id_instE {A} f : @mmap _ _ (@MMap_refl A) f = f. reflexivity. Qed.
+
+(** Simplify mmap expressions *)
+
+Ltac mmap_typeclass_normalize :=
+  repeat match goal with
+  | [|- appcontext[@mmap ?A ?B _ ?f]] =>
+     let s := constr:(@mmap A B _ f) in progress change (@mmap A B _ f) with s
+  end.
+
+Ltac mmap_typeclass_normalizeH H :=
+  repeat match typeof H with
+  | appcontext[@mmap ?A ?B _ ?f] =>
+     let s := constr:(@mmap A B _ f) in progress change (@mmap A B _ f) with s
+  end.
+
+Hint Rewrite @mmap_id_instE : mmap.
+Hint Rewrite @mmap_id @mmap_comp @mmap_idX @mmap_compX @mmap_compR
+  using exact _ : mmap.
+
+Hint Rewrite @mmap_id_instE : autosubst.
+Hint Rewrite @mmap_id @mmap_comp @mmap_idX @mmap_compX @mmap_compR
+  using exact _ : autosubst.
+
+Ltac msimpl :=
+  mmap_typeclass_normalize;
+  repeat first 
+  [ solve [trivial]
+  | progress (simpl; autorewrite with mmap)
+  | fold_id].
+
+Ltac msimplH H :=
+  mmap_typeclass_normalizeH H;
+  repeat first
+  [ solve [trivial]
+  | progress (simpl; autorewrite with mmap in H)
+  | fold_id in H].
+
+Tactic Notation "msimpl" "in" ident(H) := msimplH H.
+Tactic Notation "msimpl" "in" "*" := (in_all msimplH); msimpl.
+
+(** Deriving Instances *)
+
+Ltac derive_MMap :=
+  hnf; match goal with [ |- (?A -> ?A) -> ?B -> ?B ] =>
+    intros f; fix map 1; intros xs; change (annot B xs); destruct xs;
+    match goal with
+      | [ |- annot _ ?ys ] =>
+        let rec tmap xs :=
+            (match xs with
+               | ?s1 ?s2 =>
+                 let s1 := tmap s1 in
+                 let T  := typeof s2 in
+                 let s2 :=
+                     match T with
+                       | A => constr:(f s2)
+                       | B => constr:(map s2)
+                       | _ => constr:(mmap f s2)
+                     end in
+                 constr:(s1 s2)
+               | _ => xs
+             end) in
+        let ys := tmap ys in exact ys
+    end
+  end.
+Hint Extern 0 (MMap _ _) => derive_MMap : derive.
+
+Ltac derive_MMapLemmas := constructor;
+  [ induction 0; simpl; f_equal; trivial; apply mmap_id
+  | intros f g; induction 0; simpl; f_equal; trivial; apply mmap_comp ].
+Hint Extern 0 (MMapLemmas _ _) => derive_MMapLemmas : derive.
+
+Ltac derive_MMapExt :=
+  intros ???; fix 1; destruct 0; simpl; f_equal; auto using mmap_ext.
+Hint Extern 0 (MMapExt _ _) => derive_MMapExt : derive.
